Main.dfy
@@ -13,7 +13,7 @@ const protoTypes : map<string, Mode> :=
 
 
 
-method {:verify false} Main() {
+method {:verify false} Main1() {
 
   print "Main Test for loopback\n";
   
@@ -27,7 +27,7 @@ var t := new Object.make(protoTypes, {}, {}, "t");
 assert t.Ready();
 assert COK(t, {t});
 
-// protoTypes 8-)
+// protoTypes 8-)  
 // cat dat eye fucker jat kye lat nxt rat 
 
 var a := new Object.make(protoTypes, {t}, {t}, "a");
@@ -169,7 +169,7 @@ print "\nDone\n";
 
 
 
-method {:verify false} Main0() {
+method {:verify false} Main() {
 
 print "main showing RefOK etc\n";
   
@@ -289,6 +289,25 @@ var matrix : seq<string>:= [
          for j := 0 to |matrix[0]|
           {
          print match (inside(oq[i],oq[j]), (matrix[i][j]) )
+           case (true,  'x') => "o"  //OK, true positive
+           case (true,  ' ') => "F"  //false positive
+           case (false, ' ') => " "  //OK, true negative
+           case (false, 'x') => "M"; //false negative
+          }
+         print "\n";
+       }
+print "\n";
+
+
+
+print "ownerInsideOwner ownerInsideOwner ownerInsideOwner ownerInsideOwner\n";
+print "ownerInsideOwner ownerInsideOwner ownerInsideOwner ownerInsideOwner\n";
+
+      for i := 0 to |matrix|
+       {
+         for j := 0 to |matrix[0]|
+          {
+         print match (ownerInsideOwner(oq[i].AMFO,oq[j].AMFO), (matrix[i][j]) )
            case (true,  'x') => "o"  //OK
            case (true,  ' ') => "M"  //missing
            case (false, ' ') => " "
@@ -299,7 +318,126 @@ var matrix : seq<string>:= [
 print "\n";
 
 
+print "FUCKED FUCKED FUCKED FUCKED FUCKED\n";
+print "FUCKED FUCKED FUCKED FUCKED FUCKED\n";
 
+print "\n\nREFERENCE OK refOK =========================\n";
+print "REFERENCE OK refOK =========================\n\n";
+
+      for i := 0 to |oq|
+       {
+         print oq[i].nick;
+         //printobj(oq[i]);
+         print "  ";
+
+         for j := 0 to |oq|
+{
+         print (if (refOK(oq[i],oq[j])) then (oq[i].nick+"->"+oq[j].nick) else "    ");
+         print " ";
+}
+print "\n";
+}
+
+//uncomment to print out a new "matrix"
+// 
+// 
+//   print "\n[\n";
+// 
+//       for i := 0 to |oq|
+//        {
+//          print "\"";
+// 
+//          for j := 0 to |oq|
+// {
+//          print (if (refOK(oq[i],oq[j])) then ("x") else " ");
+// }
+//          if (i < (|oq|-1))  { print "\",\n";} else { print "\"\n";}
+// 
+//        }
+// print "]\n";
+
+
+var keanu := 
+[
+"xxxx         ",
+"xxxxxx       ",
+"xxxx         ",
+"xxxx  x  xxxx",
+"xxxxxx       ",
+"xxxxxx       ",
+"xxxx  xx xxxx",
+"xxxx  xxxxxxx",
+"xxxx  xxxxxxx",
+"xxxx  x  xxxx",
+"xxxx  x  xxxx",
+"xxxx  x  xxxx",
+"xxxx  x  xxxx"
+];
+
+
+  print "\n\n";
+
+      for i := 0 to |keanu|
+       {
+         for j := 0 to |keanu[0]|
+          {
+         print match (refOK(oq[i],oq[j]), (keanu[i][j]) )
+           case (true,  'x') => "o"  //OK, true positive
+           case (true,  ' ') => "F"  //false positive
+           case (false, ' ') => " "  //OK, true negative
+           case (false, 'x') => "M"; //false negative
+          }
+         print "\n";
+       }
+print "\n";
+
+
+print "\nDone\n\n";
+
+
+
+
+
+}
+
+// end main2
+
+
+
+
+method {:verify false} Main3() {
+
+print "main poking at bound etc\n";
+print "Object G has bound at object t\n";
+  
+var t := new Object.make(protoTypes, {}, {}, "t");
+
+//   t
+//   a       b       c
+//   d  e            f  
+//  ij kl            g 
+//                   h
+
+var a := new Object.make(protoTypes, {t}, {t},         "a");
+var b := new Object.make(protoTypes, {t}, {t},         "b");
+var c := new Object.make(protoTypes, {t}, {t},         "c");
+var d := new Object.make(protoTypes, {a}, {a,t},       "d");
+var e := new Object.make(protoTypes, {a}, {a,t},       "e");
+var f := new Object.make(protoTypes, {c}, {t,a,c},     "f");
+var g := new Object.make(protoTypes, {f}, {t,a,c,f},   "G", {t});
+var h := new Object.make(protoTypes, {g}, {t,a,c,f,g}, "H", {g});
+var i := new Object.make(protoTypes, {d}, {t,a,d},     "i");
+var j := new Object.make(protoTypes, {d}, {t,a,d},     "j");
+var k := new Object.make(protoTypes, {e}, {t,a,e},     "k");
+var l := new Object.make(protoTypes, {e}, {t,a,e},     "l");
+
+print "a->d : ", refOK(a,d), "\n";
+print "a->e : ", refOK(a,e), "\n";
+
+var os : set<Object> := {t,   a, b, c, d, e, f, g, h, i, j, k, l };
+var oq : seq<Object> := [t,   a, b, c, d, e, f, g, h, i, j, k, l ];
+
+assert forall o <- oq :: o.Ready();
 
 print "\n\nREFERENCE OK refOK =========================\n";
 print "REFERENCE OK refOK =========================\n\n";
@@ -362,10 +500,10 @@ var keanu :=
          for j := 0 to |keanu[0]|
           {
          print match (refOK(oq[i],oq[j]), (keanu[i][j]) )
-           case (true,  'x') => "o"  //OK
-           case (true,  ' ') => "M"  //missing
-           case (false, ' ') => " "
-           case (false, 'x') => "F"; //false posiutive, ie FUCKED
+           case (true,  'x') => "o"  //OK, true positive
+           case (true,  ' ') => "F"  //false positive
+           case (false, ' ') => " "  //OK, true negative
+           case (false, 'x') => "M"; //false negative
           }
          print "\n";
        }
@@ -379,9 +517,5 @@ print "\nDone\n\n";
 
 
 }
-
-
-
-// end main
 
 
